src/program_proof/mvcc/tid_proof.v
@@ -1,11 +1,16 @@
 From Perennial.base_logic Require Import ghost_map saved_prop.
+From Perennial.program_proof Require Import std_proof.
 From Perennial.program_proof.mvcc Require Import mvcc_prelude mvcc_ghost.
 From Goose.github_com.mit_pdos.go_mvcc Require Import tid.
+
+Local Ltac Zify.zify_post_hook ::= Z.div_mod_to_equations.
 
 Section program.
 Context `{!heapGS Σ, !mvcc_ghostG Σ}.
 
 Definition gentid_ns := nroot .@ "gentid".
+
+Local Definition sid_of (ts: u64) : u64 := word.modu ts (U64 N_TXN_SITES).
 
 Local Definition gentid_au (γ : mvcc_names) (sid : u64) (Φ : val → iProp Σ) : iProp Σ :=
   (|NC={⊤ ∖ ∅,∅}=>
@@ -14,7 +19,7 @@ Local Definition gentid_au (γ : mvcc_names) (sid : u64) (Φ : val → iProp Σ)
          |NC={∅,⊤ ∖ ∅}=> ∀ tid : u64, ⌜int.nat tid = ts⌝ ∗ sid_own γ sid -∗ Φ #tid)).
 
 Local Definition reserved_inv γ now (ts : u64) γr : iProp Σ :=
-  ∃ Φ, let sid := word.modu ts (U64 N_TXN_SITES) in
+  ∃ Φ, let sid := sid_of ts in
     saved_pred_own γr DfracDiscarded Φ ∗
     sid_own γ sid ∗
     if bool_decide (int.nat ts ≤ now)%nat then
@@ -25,15 +30,15 @@ Local Definition reserved_inv γ now (ts : u64) γr : iProp Σ :=
       gentid_au γ sid Φ
     .
 
-Local Definition gentid_inv (γ : mvcc_names) : iProp Σ :=
-  ∃ now (reserved : gmap u64 gname),
+Local Definition gentid_inv (γ : mvcc_names) now : iProp Σ :=
+  ∃ (reserved : gmap u64 gname),
     ts_auth γ now ∗ tsc_lb now ∗
     ghost_map_auth γ.(mvcc_gentid_reserved) 1 reserved ∗
     [∗ map] ts ↦ 'γr ∈ reserved,
       reserved_inv γ now ts γr.
 
 Definition have_gentid (γ : mvcc_names) : iProp Σ :=
-  inv gentid_ns (gentid_inv γ).
+  inv gentid_ns (∃ now, gentid_inv γ now).
 
 Local Definition tid_reserved γ γr ts (Φ : val → iProp Σ) : iProp Σ :=
   ghost_map_elem γ.(mvcc_gentid_reserved) ts (DfracOwn 1) γr ∗
@@ -45,18 +50,36 @@ Proof. apply _. Qed.
 Lemma init_GenTID γ E :
   mvcc_gentid_init γ -∗
   |={E}=> have_gentid γ.
-Proof. Admitted.
+Proof.
+  iIntros "[Hts Hres]".
+  iMod tsc_lb_0.
+  iApply inv_alloc. iNext. iExists _, ∅.
+  iFrame. rewrite big_sepM_empty. done.
+Qed.
 
-Local Lemma gentid_reserve γ sid Φ :
-  gentid_inv γ -∗
+Local Lemma gentid_reserve γ now sid Φ :
+  gentid_inv γ now -∗
   sid_own γ sid -∗
   gentid_au γ sid Φ -∗
-  |==> ∃ clock, tsc_lb clock ∗
+  |==> tsc_lb now ∗
     (* The user can pick a timestamp with the right sid, but only gets something
     out of this if they pick one that is strictly greater than [clock]. *)
-    (∀ ts, ⌜sid = word.modu ts (U64 N_TXN_SITES)⌝ ==∗
-       (if decide (clock < int.Z ts) then ∃ γr, tid_reserved γ γr ts Φ else True) ∗
-       gentid_inv γ).
+    (∀ ts, ⌜sid = sid_of ts⌝ ==∗
+       (if decide (now < int.Z ts) then ∃ γr, tid_reserved γ γr ts Φ else True) ∗
+       gentid_inv γ now).
+Proof. Admitted.
+
+Local Lemma gentid_inc_clock γ now :
+  gentid_inv γ now -∗
+  tsc_lb (now+1) -∗
+  |==> gentid_inv γ (now+1).
+Proof. Admitted.
+
+Local Lemma gentid_completed γ γr clock ts Φ :
+  gentid_inv γ clock -∗
+  tid_reserved γ γr ts Φ -∗
+  tsc_lb (int.nat ts) -∗
+  |==> ∃ clock', gentid_inv γ clock' ∗ sid_own γ (sid_of ts) ∗ gentid_au γ (sid_of ts) Φ.
 Proof. Admitted.
 
 (**
@@ -67,6 +90,7 @@ Proof. Admitted.
 (* func GenTID(sid uint64) uint64                                *)
 (*****************************************************************)
 Theorem wp_GenTID (sid : u64) γ :
+  int.Z sid < N_TXN_SITES →
   ⊢ have_gentid γ -∗
     {{{ sid_own γ sid }}}
     <<< ∀∀ (ts : nat), ts_auth γ ts >>>
@@ -74,7 +98,7 @@ Theorem wp_GenTID (sid : u64) γ :
     <<< ∃ ts', ts_auth γ ts' ∗ ⌜(ts < ts')%nat⌝ >>>
     {{{ (tid : u64), RET #tid; ⌜int.nat tid = ts⌝ ∗ sid_own γ sid }}}.
 Proof.
-  iIntros "#Hinv !>" (Φ) "Hsid HAU".
+  iIntros "%Hsid #Hinv !>" (Φ) "Hsid HAU".
   wp_call.
 
   (***********************************************************)
@@ -90,34 +114,62 @@ Proof.
   (***********************************************************)
   wp_apply (wp_GetTSC).
   iInv "Hinv" as "Hgentid" "Hclose".
-  iMod (lc_fupd_elim_later with "LC Hgentid") as "Hgentid".
-  iMod (gentid_reserve with "Hgentid Hsid HAU") as (clock) "[Hclock Hcont]".
+  iMod (lc_fupd_elim_later with "LC Hgentid") as (clock) "Hgentid".
+  iMod (gentid_reserve with "Hgentid Hsid HAU") as "[Hclock Hcont]".
   iApply ncfupd_mask_intro.
   { solve_ndisj. }
   iIntros "Hclose2".
   iExists _. iFrame "Hclock".
   iIntros (clock2) "[%Hclock Hclock2]".
   iMod "Hclose2" as "_".
-  set reserved_ts := word.add clock2 (U64 1). (* FIXME use the actual ID here *)
+  set inbounds := bool_decide (int.Z clock2 + 64 < 2^64).
+  set clock2_boundsafe := if inbounds then clock2 else 0.
+  feed pose proof (u64_round_up_spec clock2_boundsafe (U64 64)) as H.
+  { subst clock2_boundsafe inbounds. case_bool_decide; word. }
+  { word. }
+  move:H.
+  set rounded_ts := u64_round_up clock2_boundsafe (U64 64).
+  intros (Hmod & Hbound1 & Hbound2).
+  set reserved_ts := word.add rounded_ts sid.
+  assert ((int.Z rounded_ts + int.Z sid) `mod` 64 = int.Z sid) as Hsidmod.
+  { rewrite Z.add_mod. 2:lia.
+    rewrite Hmod. rewrite [int.Z sid `mod` _]Z.mod_small. 2:split;[word|done].
+    rewrite Z.mod_small. 1:lia. split;[word|done]. }
+  assert (int.Z (sid_of reserved_ts) = int.Z sid) as Hsid_of.
+  { rewrite /sid_of /reserved_ts.
+    rewrite word.unsigned_modu. 2:done.
+    rewrite word.unsigned_add. rewrite (wrap_small (_+_)). 2:word.
+    rewrite wrap_small. 1:done.
+    split.
+    - apply Z_mod_nonneg_nonneg. all:try word. all:done.
+    - trans (int.Z N_TXN_SITES). 2:done. apply Z.mod_pos_bound. done.
+  }
   iMod ("Hcont" $! reserved_ts with "[]") as "[Hreserved Hgentid]".
-  { iPureIntro. admit. }
-  iMod ("Hclose" with "Hgentid") as "_".
+  { iPureIntro. rewrite /sid_of /reserved_ts. apply word.unsigned_inj. done. }
+  iMod ("Hclose" with "[Hgentid]") as "_".
+  { eauto. }
   iIntros "!> _".
 
   (************************************************************************)
-  (* tid = ((tid + config.N_TXN_SITES) & ^(config.N_TXN_SITES - 1)) + sid *)
+  (* tid = ... *)
   (************************************************************************)
   wp_store.
   wp_load.
+  wp_apply wp_SumAssumeNoOverflow. iIntros (Hoverflow).
+  assert (inbounds = true) as ->.
+  { subst inbounds. rewrite bool_decide_true; first done. word. }
+  subst clock2_boundsafe.
   wp_store.
   wp_pures.
+
   set tid := (word.add _ _).
+  assert (tid = reserved_ts) as -> by done.
 
   (***********************************************************)
   (* for GetTSC() <= tid {                                   *)
   (* }                                                       *)
   (***********************************************************)
-  set P := λ (b : bool), (if b then True else tsc_lb (int.nat tid))%I.
+  set P := λ (b : bool), (if b then True else tsc_lb (int.nat reserved_ts))%I.
   wp_apply (wp_forBreak_cond P).
   { admit. }
   { done. }
